

```

In[37]:= M3 = {{-(ℓ c γ) - c Subscript[r, x], c Subscript[r, x]},
              {β (1 - ℓ c γ - c Subscript[r, x]), -β + β c Subscript[r, x]}};
M3 // MatrixForm
{val, vec} = Eigensystem[M3];
val[[2]] (* The eigenvalue of M1 *)
{1, vec[[2]] [[2]] / vec[[2]] [[1]]} (* Corresponding eigenvector *)

Out[38]//MatrixForm=

$$\begin{pmatrix} -c \ell \gamma - c r_x & c r_x \\ \beta (1 - c \ell \gamma - c r_x) & -\beta + c \beta r_x \end{pmatrix}$$


Out[40]=

$$\frac{1}{2} \left( -\beta - c \ell \gamma - c r_x + c \beta r_x + \sqrt{-4 c \ell \beta \gamma + (\beta + c \ell \gamma + c r_x - c \beta r_x)^2} \right)$$


Out[41]=

$$\left\{ 1, \right. \\ \left. - \left( (2 \beta (-1 + c \ell \gamma + c r_x)) / (\beta - c \ell \gamma - c r_x - c \beta r_x + \sqrt{\beta^2 - 2 c \ell \beta \gamma + c^2 \ell^2 \gamma^2 + 2 c \beta r_x - 2 c \beta^2 r_x + 2 c^2 \ell \gamma r_x - 2 c^2 \ell \beta \gamma r_x + c^2 r_x^2 - 2 c^2 \beta r_x^2 + c^2 \beta^2 r_x^2}) \right) \right\}$$


In[42]:= A3 := ℓ c γ + c Subscript[r, x];
B3 := 1 - c Subscript[r, x];
Simplify[val[[2]] - (-A3 / 2 - (B3 β) / 2 + (1 / 2) Sqrt[(A3 + B3 β) ^ 2 - 4 ℓ c β γ]]
(* Check the form of λ *)
Simplify[vec[[2]] - ({(1 / (2 (1 - A3) β)) *
  (-A3 + B3 β + Sqrt[(A3 - B3 β) ^ 2 + 4 c Subscript[r, x] β (1 - A3)]), 1}
  (* Check the form of corresponding eigenvector. *)
)]

Out[44]=
0

Out[45]=
{0, 0}

```